Simplify the term language even further

src/Denote.v
@@ -14,7 +14,6 @@ Require Import Category.Theory.Functor.
 
 Require Import Solver.Lib.
 Require Import Solver.Expr.
-Require Import Solver.Normal.
 
 Generalizable All Variables.
 
@@ -27,30 +26,39 @@ Variable arrs : ∀ f : arr_idx, option (∃ x y, objs x ~{C}~> objs y).
 
 Import EqNotations.
 
-Fixpoint termD dom cod (e : Term) : option (objs dom ~{C}~> objs cod) :=
+Fixpoint termD_work dom (e : Term) : option (∃ cod, objs dom ~{C}~> objs cod) :=
   match e with
-  | Identity _ =>
-      match Eq_eq_dec cod dom with
-      | left edom =>
-        Some (rew [fun x => objs x ~{ C }~> objs cod] edom in @id _ (objs cod))
-      | right _ => None
-      end
-  | Morph _ _ a =>
+  | Identity => Some (dom; @id _ (objs dom))
+  | Morph a =>
     match arrs a with
-    | Some (x'; (y'; f)) =>
-      match Eq_eq_dec x' dom, Eq_eq_dec y' cod with
-      | left edom, left ecod =>
-        Some (rew [fun x => objs x  ~{ C }~> objs cod] edom in
-              rew [fun y => objs x' ~{ C }~> objs y] ecod in f)
-      | _, _ => None
+    | Some (x; (y; f)) =>
+      match Eq_eq_dec x dom with
+      | left edom =>
+        Some (y; rew [fun x => objs x  ~{ C }~> objs y] edom in f)
+      | _ => None
       end
     | _ => None
     end
-  | Compose mid f g =>
-    match termD mid cod f, termD dom mid g with
-    | Some f, Some g => Some (f ∘ g)
-    | _, _ => None
+  | Compose f g =>
+    match termD_work dom g with
+    | Some (mid; g) =>
+      match termD_work mid f with
+      | Some (y; f) => Some (y; f ∘ g)
+      | _ => None
+      end
+    | _ => None
     end
+  end.
+
+Definition termD dom cod (e : Term) : option (objs dom ~{C}~> objs cod) :=
+  match termD_work dom e with
+  | Some (y; f) =>
+    match Eq_eq_dec y cod with
+    | left ecod =>
+        Some (rew [fun y => objs dom ~{ C }~> objs y] ecod in f)
+    | right _ => None
+    end
+  | _ => None
   end.
 
 Fixpoint exprD (e : Expr) : Type :=
@@ -58,85 +66,9 @@ Fixpoint exprD (e : Expr) : Type :=
   | Top           => True
   | Bottom        => False
   | Equiv x y f g => termD x y f ≈ termD x y g
-  (* | Not p         => exprD p -> False *)
   | And p q       => exprD p ∧ exprD q
   | Or p q        => exprD p + exprD q
   | Impl p q      => exprD p -> exprD q
   end.
-
-Fixpoint arrowsD dom cod `(fs : list (Arrow t)) :
-  option (objs dom ~{C}~> objs cod) :=
-  match fs with
-  | nil =>
-    match Eq_eq_dec cod dom with
-    | left edom =>
-      Some (rew [fun x => objs x ~{ C }~> objs cod] edom in @id _ (objs cod))
-    | right _ => None
-    end
-  | cons f nil =>
-    match arrs (snd (get_arrow f)) with
-    | Some (x'; (y'; f)) =>
-      match Eq_eq_dec x' dom, Eq_eq_dec y' cod with
-      | left edom, left ecod =>
-        Some (rew [fun x => objs x  ~{ C }~> objs cod] edom in
-              rew [fun y => objs x' ~{ C }~> objs y] ecod in f)
-      | _, _ => None
-      end
-    | _ => None
-    end
-  | cons f fs =>
-    let '(x, a) := get_arrow f in
-    match arrowsD dom x fs with
-    | Some g =>
-      match arrs a with
-      | Some (x'; (y'; f)) =>
-        match Eq_eq_dec x' x, Eq_eq_dec y' cod with
-        | left edom, left ecod =>
-          Some (rew [fun x => objs x  ~{ C }~> objs cod] edom in
-                rew [fun y => objs x' ~{ C }~> objs y] ecod in f ∘ g)
-        | _, _ => None
-        end
-      | _ => None
-      end
-    | _ => None
-    end
-  end.
-
-Fixpoint exprAD (e : Expr) : Type :=
-  match e with
-  | Top           => True
-  | Bottom        => False
-  | Equiv x y f g => arrowsD x y (arrows f) ≈ arrowsD x y (arrows g)
-  (* | Not p         => exprD p -> False *)
-  | And p q       => exprD p ∧ exprD q
-  | Or p q        => exprD p + exprD q
-  | Impl p q      => exprD p -> exprD q
-  end.
-
-Theorem arrowsD_sound {p dom cod f} :
-  arrowsD dom cod (arrows p) = Some f ->
-  ∃ f', f ≈ f' ∧ termD dom cod p = Some f'.
-Proof.
-Admitted.
-
-Lemma arrowsD_apply dom cod (f g : Term) :
-  arrows_bequiv (arrows f) (arrows g) = true ->
-  arrowsD dom cod (arrows f) ||| false = true ->
-  arrowsD dom cod (arrows f) = arrowsD dom cod (arrows g) ->
-  termD dom cod f ≈ termD dom cod g.
-Proof.
-  intros.
-  destruct (arrowsD dom cod (arrows f)) eqn:?; [|discriminate].
-  destruct (arrowsD_sound Heqo), p.
-  rewrite e0; clear e0.
-  rewrite H1 in Heqo; clear H1.
-Admitted.
-
-Lemma exprAD_sound (e : Expr) : exprAD e -> exprD e.
-Proof.
-  destruct e; auto; intros.
-  red in X; red.
-  apply arrowsD_apply; auto.
-Abort.
 
 End Denote.
