src/Normal.v
@@ -20,17 +20,26 @@ Generalizable All Variables.
 
 Section Normal.
 
+Context {C : Category}.
+
+Variable objs : obj_idx -> C.
+Variable arrs : ∀ f : arr_idx, option (∃ x y, objs x ~{C}~> objs y).
+
+Import EqNotations.
+
+(*
 Inductive Arrow : Term -> Set :=
-  | Here  : ∀ x y a, Arrow (Morph x y a)
-  | Left  : ∀ (m : obj_idx) f g, Arrow f -> Arrow (Compose m f g)
-  | Right : ∀ (m : obj_idx) f g, Arrow g -> Arrow (Compose m f g).
+
+  | Here  : ∀ a, Arrow (Morph a)
+  | Left  : ∀ f g, Arrow f -> Arrow (Compose f g)
+  | Right : ∀ f g, Arrow g -> Arrow (Compose f g).
 
 Definition Arrow_inv_t : forall t, Arrow t -> Type.
 Proof.
   intros [] H.
   - exact False.
-  - exact (H = Here x y a).
-  - exact ((∃ H', H = Left m f g H') + (∃ H', H = Right m f g H')).
+  - exact (H = Here a).
+  - exact ((∃ H', H = Left f g H') + (∃ H', H = Right f g H')).
 Defined.
 
 Lemma Arrow_inv t f : Arrow_inv_t t f.
@@ -40,18 +49,18 @@ Proof.
   - right. exists f0; auto.
 Defined.
 
-Lemma Arrow_Morph `(H : Arrow (Morph x y a)) : H = Here x y a.
+Lemma Arrow_Morph `(H : Arrow (Morph a)) : H = Here a.
 Proof. exact (Arrow_inv _ H). Defined.
 
-Lemma Arrow_Compose `(H : Arrow (Compose m f g)) :
-  (∃ H', H = Left m f g H') + (∃ H', H = Right m f g H').
+Lemma Arrow_Compose `(H : Arrow (Compose f g)) :
+  (∃ H', H = Left f g H') + (∃ H', H = Right f g H').
 Proof. exact (Arrow_inv _ H). Defined.
 
-Fixpoint get_arrow `(f : Arrow t) : obj_idx * arr_idx :=
+Fixpoint get_arrow `(f : Arrow t) : arr_idx :=
   match f with
-  | Here x _ a    => (x, a)
-  | Left _ _ _ x  => get_arrow x
-  | Right _ _ _ x => get_arrow x
+  | Here a      => a
+  | Left _ _ x  => get_arrow x
+  | Right _ _ x => get_arrow x
   end.
 
 Function arrow_bequiv {t t' : Term} (p : Arrow t) (q : Arrow t') : bool :=
@@ -74,6 +83,65 @@ Function arrows_bequiv {t t' : Term}
   | cons p ps, cons q qs =>
     arrow_bequiv p q &&& arrows_bequiv ps qs
   | _, _ => false
+  end.
+*)
+
+Function arrows (t : Term) : list arr_idx :=
+  match t with
+  | Identity    => nil
+  | Morph a     => [a]
+  | Compose f g => arrows f ++ arrows g
+  end.
+
+Fixpoint arrowsD_work dom (fs : list arr_idx) :
+  option (∃ cod, objs dom ~{C}~> objs cod) :=
+  match fs with
+  | nil => Some (dom; @id _ (objs dom))
+  | a :: fs =>
+    match arrs a with
+    | Some (x; (y; f)) =>
+      match fs with
+      | nil =>
+        match Eq_eq_dec x dom with
+        | left edom =>
+          Some (y; rew [fun x => objs x ~{ C }~> objs y] edom in f)
+        | _ => None
+        end
+      | _ =>
+        match arrowsD_work dom fs with
+        | Some (mid; g) =>
+          match Eq_eq_dec mid x with
+          | left emid =>
+            Some (y; f ∘ rew [fun y => objs dom ~{ C }~> objs y] emid in g)
+          | _ => None
+          end
+        | _ => None
+        end
+      end
+    | _ => None
+    end
+  end.
+
+Fixpoint arrowsD dom cod (fs : list arr_idx) :
+  option (objs dom ~{C}~> objs cod) :=
+  match arrowsD_work dom fs with
+  | Some (y; f) =>
+    match Eq_eq_dec y cod with
+    | left ecod =>
+      Some (rew [fun y => objs dom ~{ C }~> objs y] ecod in f)
+    | right _ => None
+    end
+  | _ => None
+  end.
+
+Fixpoint exprAD (e : Expr) : Type :=
+  match e with
+  | Top           => True
+  | Bottom        => False
+  | Equiv x y f g => arrowsD x y (arrows f) ≈ arrowsD x y (arrows g)
+  | And p q       => exprAD p ∧ exprAD q
+  | Or p q        => exprAD p + exprAD q
+  | Impl p q      => exprAD p -> exprAD q
   end.
 
 End Normal.
