src/Sound.v
@@ -1,0 +1,56 @@
+Set Warnings "-notation-overridden".
+
+Require Import Coq.Program.Program.
+Require Import Coq.Bool.Bool.
+Require Import Coq.Arith.Bool_nat.
+Require Import Coq.Arith.PeanoNat.
+Require Import Coq.PArith.PArith.
+Require Import Coq.Lists.List.
+Require Import Coq.omega.Omega.
+Require Import Coq.Wellfounded.Lexicographic_Product.
+Require Import Recdef.
+
+Require Import Category.Lib.
+Require Import Category.Theory.Functor.
+
+Require Import Solver.Lib.
+Require Import Solver.Expr.
+Require Import Solver.Denote.
+Require Import Solver.Normal.
+
+Generalizable All Variables.
+
+Section Normal.
+
+Context {C : Category}.
+
+Variable objs : obj_idx -> C.
+Variable arrs : ∀ f : arr_idx, option (∃ x y, objs x ~{C}~> objs y).
+
+Theorem arrowsD_sound {p dom cod f} :
+  arrowsD objs arrs dom cod (arrows p) = Some f ->
+  ∃ f', f ≈ f' ∧ termD objs arrs dom cod p = Some f'.
+Proof.
+Admitted.
+
+Lemma arrowsD_apply dom cod (f g : Term) :
+  list_beq Eq_eqb (arrows f) (arrows g) = true ->
+  arrowsD objs arrs dom cod (arrows f) ||| false = true ->
+  arrowsD objs arrs dom cod (arrows f) = arrowsD objs arrs dom cod (arrows g) ->
+  termD objs arrs dom cod f ≈ termD objs arrs dom cod g.
+Proof.
+  intros.
+  destruct (arrowsD objs arrs dom cod (arrows f)) eqn:?; [|discriminate].
+  destruct (arrowsD_sound Heqo), p.
+  rewrite e0; clear e0.
+  rewrite H1 in Heqo; clear H1.
+Admitted.
+
+Lemma exprAD_sound (e : Expr) : exprAD objs arrs e -> exprD objs arrs e.
+Proof.
+  destruct e; auto; intros.
+  red in X; red.
+  apply arrowsD_apply; auto.
+Abort.
+
+End Normal.
